## Lecture 13: Algerbra 101 Follow the rules

### Basic rules
* Commutative law $a+b=b+a$
* Associative law $a+(b+c)=(a+b)+c$
* Distributive law $a(b+c)=ab+ac$, $(a+b)c=ac+bc$
* Negation law $-a=(-1)a$
* numbers before variables $3x$ not $x3$


**Example**
* easy ones
$$
\begin{aligned}
a-(b+c)& =a+(-1)(b+c) \\
&=a+((-1)b+(-1)c)\\
&=a-b-c
\end{aligned}$$

$$
\begin{aligned}
a-(b-c)& =a+(-1)(b-c) \\
&=a+((-1)b-(-1)c)\\
&=a-b+c
\end{aligned}$$

$$
\begin{aligned}
4a-3-2(a+1)& =4a-3-2a-2 \\
&=2a-5
\end{aligned}$$

* more work
$$\begin{aligned}
(a+2)(a+1)& =a(a+1)+2(a+1) \\
&=a^2+a+2a+2\\
&=a^2+3a+2
\end{aligned}$$

$$\begin{aligned}
(a+b)(a-b)& =a(a-b)+b(a-b) \\
&=a^2-ab+ba-b^2\\
&=a^2-b^2
\end{aligned}$$

$$\begin{aligned}
(a+b)^2=(a+b)(a+b)& =a(a+b)+b(a+b) \\
&=a^2+ab+ba+b^2\\
&=a^2+2ab+b^2
\end{aligned}$$

$$\begin{aligned}
(a-b)^2&= (a+(-b))^2 \\
&=a^2+2a(-b)+(-b)^2\\
&=a^2-2ab+b^2
\end{aligned}$$

$$\begin{aligned}
(2a-4)^2&=(2a)^2-2(2a)(-4)+(-4)^2\\
&=4a^2+16a+16
\end{aligned}$$

* In general, we have 
$$\begin{aligned}
(a+b)(c+d)& =a(c+d)+b(c+d) \\
&=ac+ad+bc+bd
\end{aligned}$$

* Applications:
$$\begin{aligned}
101^2&=(100+1)^2\\
&=10000+200+1=10201
\end{aligned}$$

$$\begin{aligned}
100^2-99^2&=(100+99)(100-99)\\
&=199
\end{aligned}$$

* more and more work
$$\begin{aligned}
(a+b)^3&= (a+b)(a+b)^2 \\
&=(a+b)(a^2+2ab+b^2)\\
&=a(a^2+2ab+b^2)+b(a^2+2ab+b^2)\\
&=a^3+2a^2b+ab^2+ba^2+2ab^2+b^3\\
&=a^3+3a^2b+3ab^2+b^3
\end{aligned}$$

$$\begin{aligned}
(a+b)^4&= (a+b)(a^3+3a^2b+3ab^2+b^3) \\
&=a(a^3+3a^2b+3ab^2+b^3)+b(a^3+3a^2b+3ab^2+b^3)\\
&=a^4+3a^3b+3a^2b^2+ab^3+ba^3+3a^2b^2+3ab^3+b^4\\
&=a^4+4a^3b+6a^2b^2+4ab^3+b^4
\end{aligned}$$

**Why?** Pascal's triangle?? Pick $k$ of $b$'s out of the product.  

$$(a+b)^n=a^n+\binom{n}{1}a^{n-1}b+\binom{n}{2}a^{n-2}b^2+...+\binom{n}{n-1}ab^{n-1}+b^n$$

* more and more work
$$\begin{aligned}
(a+b+c)^2&= ((a+b)+c)^2 \\
&=(a+b)^2+2(a+b)c+c^2\\
&=a^2+2ab+b^2+2ac+2bc+c^2\\
&=a^2+b^2+c^2+2ab+2ac+2bc
\end{aligned}$$

### Factorization 
A polynomial $p(x)$ in one variable is of the form with $x$ and its powers in such as:
$$x+3,2x-5,3x^2+4x+1,x^{5}-1,...$$

A facorization means the polynomial is expressed as a product of linear terms.

$$x^2-4=(x-2)(x+2)$$

$$x^2-2x-3=(x-3)(x+1)$$

If you can factor a quadratic polynomial, you can find the solution of $p(x)=0$. The general quadratic polynomial is of the form 
$$ax^2+bx+c=a(x^2+\frac{b}{a}x+\frac{c}{a})$$

We will start with $a=1$. Let us pretend 


$$\begin{aligned}
x^2+bx+c&=(x-x_1)(x-x_2)\\
&=x^2-(x_1+x_2)x+x_1x_2
\end{aligned}$$

In particular, we get a special form of Vieta's formula:

$$c=x_1x_2$$

$$b=-(x_1+x_2)$$

Now it is a guess game

**Examples**:
* $p(x)=x^2-2x-3$, $-3$ as a product, $(-1)*3$ or $(-3)*1$, so must be $(x-3)(x-(-1))$
* $x^2+25x+84$, factor $84=4*21$, so we have $(x+4)(x+21)$
* $x^2-7x+10$, factor $10$ as two and sum up to $7$, so $(x-2)(x-5)$
* $x^2-9x+9$, perfect square, use $(a-b)^2$, we get $(x-3)^2$
* $x^2-36$, use $a^2-b^2$, so $(x-6)(x+6)$


**More difficult examples**
Guess the product. 

* $9x^2+6x+1=(3x+1)(3x+1)$
* $6x^2-23x-18=(2x-9)(3x+2)$
